

# ODE Midterm

Ata Berk Saraç

April 2025

**Question 1.** Solve the following first order differential equations:

(a)  $\cos(x)dy = y(\sin(x) - y)dx$ ,

(b)  $(2x + y - 3)dy = (x + 2y - 3)dx$ .

*Solution.* (a) This D.E. turns into

$$y' - \tan(x)y = -\sec(x)y^2,$$

we recognize that it is a Bernoulli D.E. It follows that

$$y^{-2}y' - \tan(x)y^{-1} = -\sec(x),$$

substituting  $v = y^{-1}$ , we have  $v' = -y^{-2}y'$  and so

$$v' + \tan(x)v = \sec(x)$$

which is a linear D.E.

Consider a function  $\mu(x)$  such that  $\mu'(x) = \mu(x)\tan(x)$

$$\mu(x)v' + \mu'(x)v = \mu(x)\sec(x).$$

Therefore,  $\mu(x) = e^{\int \tan(x) dx}$  so that  $\mu(x) = e^{-\ln|\cos(x)|} = \sec(x)$ . Thus,

$$v(x) = \frac{\int \sec^2(x) dx + c}{\sec(x)} = \frac{\tan(x) + c}{\sec(x)} = \sin(x) + c \cos(x)$$

so that

$$y(x) = \frac{1}{\sin(x) + c \cos(x)}$$

where  $c$  is a constant.

(b) Let  $u = x - 1$  and  $v = y - 1$ . Then

$$\frac{dv}{du} = \frac{u + 2v}{2u + v}$$

Assume that  $z = \frac{v}{u}$ , then  $v' = z + uz'$ ; therefore

$$u \frac{dz}{du} = \frac{1 - z^2}{2 + z}.$$

It follows that

$$\int \frac{1}{1+z} dz - \int \frac{-1}{1-z} dz - \frac{1}{2} \int \frac{-2z}{1-z^2} dz = \int \frac{1}{u} du,$$

thus

$$\ln|1+z| - \ln|1-z| - \frac{1}{2} \ln|1-z^2| = \ln\left|\frac{1+z}{(1-z)^2}\right| = \ln|u| + C,$$

we get

$$\frac{1}{1-z} = Cu,$$

and finally

$$z = 1 - \frac{1}{Cu}.$$

Now, we rearrange the equation above

$$\frac{y-1}{x-1} = 1 - \frac{1}{C(x-1)}$$

to get

$$y(x) = x - \frac{1}{C}$$

where  $C$  is an arbitrary constant.

**Question 2.** Show that  $y = 1 - 4x$  is a particular solution of  $y' = y^2 + 8xy + 16x^2 - 5$ , and find its general solution.

*Solution.* Call  $y, y_p$ ; then  $y_p = 1 - 4x$  and  $y'_p = -4$ . We check the validity of  $y_p$  as a solution:

$$y'_p = y_p^2 + 8xy_p + 16x^2 - 5 = (1-4x)^2 + 8x(1-4x) + 16x^2 - 5 = 1 - 8x + 16x^2 + 8x - 32x^2 + 16x^2 - 5 = -4,$$

therefore  $y_p$  is in fact a particular solution for our D.E.

Observe that  $y' = y^2 + 8xy + 16x^2 - 5$  is a Riccati D.E. which can be turned into the form  $(y + 4x)^2 - 5$ . So, let  $u = y + 4x$ . Since  $u' = y' + 4$ , we have  $\frac{du}{dx} = u^2 - 1$  and so  $\frac{du}{u^2-1} = dx$  which is a separable equation.

It follows that

$$\int \frac{du}{u^2-1} = \frac{1}{2} \int \left( \frac{1}{u-1} - \frac{1}{u+1} \right) du = \frac{1}{2} \ln \left| \frac{u-1}{u+1} \right| = x + C,$$

so that

$$\frac{u-1}{u+1} = Ke^{2x}$$

where  $K = e^{2C}$ .

We have that

$$\begin{aligned} u-1 &= Ke^{2x}(u+1), \\ u(x) &= \frac{1+K^{2x}}{1-K^{2x}}, \end{aligned}$$

thus

$$y(x) = \frac{1+K^{2x}}{1-K^{2x}} - 4x,$$

where  $K \in \mathbb{R}$  is an arbitrary constant.

**Question 3.** Show that  $y_1 = 3x^2 - 1$  is a solution. Find the general solution of

$$(1-x^2)y'' - 2xy' + 6y = 0. (*)$$

*Solution.* Note that  $y'_1 = 6x$  and  $y''_1 = 6$ . It follows that

$$(1-x^2)6 - 2x \cdot 6x + 6(3x^2-1) = 6 - 6x^2 - 12x^2 + 18x^2 - 6 = 0.$$

We can rewrite (\*) as

$$y'' - \frac{2x}{1-x^2}y' + \frac{6}{1-x^2}y = 0.$$

Now, we look for a second solution  $y_2(x)$  such that

$$y_2(x) = v(x)y_1(x)$$

where  $v(x)$  is a first-order D.E. Compute

$$y'_2 = v'y_1 + vy'_1, \quad y''_2 = v''y_1 + 2(v'y'_1) + vy''_1;$$

therefore

$$[v''y_1 + 2(v'y'_1) + vy''_1] - \frac{2x}{1-x^2}[v'y_1 + vy'_1 + 6xv] + \frac{6}{1-x^2}[vy_1] = 0.$$

Since  $y_1$  itself satisfies (\*), all the terms proportional to  $v$  cancel out so letting  $P(x) = \frac{2x}{1-x^2}$ , we are left with

$$[v''y_1 + 2(v'y'_1)] - P[v'y_1] = 0.$$

Set  $w(x) = v'(x)$ . The equation above turns into

$$w'y_1 + (y'_1 - Py_1)w = 0 \implies \frac{dw}{dx} + \left( \frac{y'_1}{y_1} - P \right)w = 0$$

which is a first order linear D.E.

**Question 4.** Find an integrating factor in terms of  $u = x^2 + y^2$  for the differential equation and then solve it:

$$(x^3 + xy^2 - y)dx + xdy = 0.$$

*Solution.* Note that  $\frac{du}{dx} = 2x$  and  $\frac{du}{dy} = 2y$ . The equation is not exact since  $\frac{\partial M}{\partial y} = 2xy - 1$  and  $\frac{\partial N}{\partial x} = 1$ .

$$\begin{aligned}\frac{\mu'(u)}{\mu(u)} &= \frac{\frac{\partial N}{\partial x} - \frac{\partial M}{\partial y}}{2yM - 2xN} \\ &= \frac{1 - (2xy - 1)}{2y(x^3 + xy^2 - y) - 2x^2} \\ &= \frac{2(1 - xy)}{2(xy - 1)(x^2 + y^2)} \\ &= \frac{-1}{x^2 + y^2},\end{aligned}$$

thus

$$\mu(u) = e^{-\int \frac{1}{u} du} = e^{-\ln|u|} = \frac{1}{u} = \frac{1}{x^2 + y^2}.$$

Multiplying by the integrating factor, the equation becomes:

$$\left(x - \frac{y}{x^2 + y^2}\right)dx + \frac{x}{x^2 + y^2}dy = 0.$$

Now,  $\frac{\partial M'}{\partial y} = \frac{\partial N'}{\partial x} = -\frac{x^2 - y^2}{(x^2 + y^2)^2}$ , confirming exactness. Integrate  $M'$  with respect to  $x$  to get

$$\frac{x^2}{2} - \arctan\left(\frac{x}{y}\right) + h(y).$$

Differentiate with respect to  $y$  and solve for  $h(y)$  to find  $h(y)$  is constant. Thus, the solution is:

$$\frac{x^2}{2} - \arctan\left(\frac{x}{y}\right) = C.$$

**Question 5.** Find the orthogonal curves of the family  $y = -x - 1 + ce^x$  (\*).

*Solution.* We have  $\frac{dy}{dx} = ce^x - 1$  (\*), adding  $- (*)$  and  $(\cdot)$  we get

$$\begin{aligned}\frac{dy}{dx} &= x + y, \\ \frac{dy}{dx}\Big|_{\text{orth}} &= -\frac{1}{\frac{dy}{dx}} = -\frac{1}{x + y},\end{aligned}$$

thus

$$\frac{dx}{dy} = -x - y$$

is orthogonal to the curves defined by (\*).

Then,

$$\frac{dx}{dy} + x = -y$$

which is a first order linear D.E., it follows that the integrating factor

$$\mu(y) = e^{\int 1 dy} = e^y,$$

multiply all terms by  $\mu(y)$

$$e^y \frac{dx}{dy} + e^y x = \frac{d}{dy}(xe^y) = -e^y y.$$

Integrate with respect to  $y$

$$xe^y = -\int ye^y dy + K = (1 - y)e^y + K$$

so that

$$x = 1 - y + Ke^{-y}$$

is a family of curves orthogonal to the family (\*).

**Question 6.** Let  $y_1, y_2, \dots, y_n$  be  $n$  solutions of the homogeneous linear  $n$ -th order differential equation on an interval  $I$ . Then the set of solutions is linearly independent on  $I$  if and only if  $W(y_1, y_2, \dots, y_n) \neq 0$  for every  $x$  in the interval.

*Solution.* Suppose, to the contrary, that  $W(y_1, y_2, \dots, y_n)(x_0) \neq 0$  at some point  $x_0 \in I$  but the  $y_i$  are linearly dependent. Then there exist constants  $c_1, \dots, c_n$ , not all zero, so that

$$c_1 y_1(x) + \dots + c_n y_n(x) = 0$$

on  $I$ .

Differentiating  $n - 1$  times gives a homogeneous linear system

$$\begin{bmatrix} y_1(x_0) & \cdots & y_n(x_0) \\ y_1'(x_0) & \cdots & y_n'(x_0) \\ \vdots & & \vdots \\ y_1^{(n-1)}(x_0) & \cdots & y_n^{(n-1)}(x_0) \end{bmatrix} \begin{bmatrix} c_1 \\ \vdots \\ c_n \end{bmatrix} = 0.$$

Call the matrices on the left-hand side  $W$  and  $c$  respectively. A nontrivial solution  $c$  exists only if  $W$  has determinant zero, since if  $W$  had nonzero determinant, then it would be invertible, so that  $W^{-1}Wc = c = 0$ . But its determinant is exactly  $W(y_1, y_2, \dots, y_n)(x_0)$ , which we assumed nonzero, a contradiction! Thus,  $W(y_1, y_2, \dots, y_n)(x) \neq 0$  implies that the set of solutions is linearly independent on  $I$ .

Now, assume that the set of solutions is linearly independent on  $I$ . It follows that there exist  $a_i$  corresponding to each  $y_i$  such that

$$\sum_{i=1}^n a_i y_i = 0,$$

differentiating one times we get

$$\sum_{i=1}^n a_i y_i' = 0$$

and so on. We thus obtain that all columns are linearly independent, meaning that the rank of the matrix is  $n$ , since row and column ranks are equal, row rank is also  $n$  which implies that the determinant of this matrix must be nonzero. The result follows.

**Question 7.** Find the general solution of the following differential equations:

(a)  $y^{(4)} + 8y'' + 16y = 0$ ,

(b)  $9y'' + 6y' + 5y = 0$ .

*Solution.* (a) Assume a solution of the form  $y = e^{rx}$ , then  $y^{(i)} = r^i e^{rx}$  for  $i \in \mathbb{N}$ . Substituting, our equation becomes

$$r^4 e^{rx} + 8r^2 e^{rx} + 16e^{rx} = 0,$$

since  $e^{rx} \neq 0$ , we get

$$r^4 + 8r^2 + 16 = 0.$$

Now, let  $u = r^2$ . The equation becomes

$$u^2 + 8u + 16 = (u + 4)^2 = 0.$$

So,  $u = -4$  is a repeated root of multiplicity 2, and so  $r = \pm\sqrt{-4} = \pm 2i$ , following that  $r = +2i$  and  $r = -2i$  are both repeated roots of multiplicity 2. The repeated roots  $r = \pm 2i$  (each with multiplicity 2) lead to the general solution:

$$y(x) = (C_1 + C_2 x) \cos(2x) + (C_3 + C_4 x) \sin(2x),$$

where  $C_1, C_2, C_3, C_4$  are constants.

(b) For the differential equation  $9y'' + 6y' + 5y = 0$ , we solve the characteristic equation  $9r^2 + 6r + 5 = 0$ . Using the quadratic formula:

$$r = \frac{-6 \pm \sqrt{36 - 180}}{18} = \frac{-6 \pm 12i}{18} = -\frac{1}{3} \pm \frac{2}{3}i.$$

The general solution with complex roots  $\alpha \pm \beta i$  is:

$$(x) = e^{-\frac{x}{3}} \left( C_1 \cos\left(\frac{2x}{3}\right) + C_2 \sin\left(\frac{2x}{3}\right) \right),$$

where  $C_1, C_2$  are constants.